did some Auction stuff

examples/auction/Auction.v
@@ -1,6 +1,7 @@
 From Coq Require Import Bool.
 From Coq Require Import ZArith_base.
 From Coq Require Import List. Import ListNotations.
+From Coq Require Import String.
 From ConCert.Execution Require Import Blockchain.
 From ConCert.Execution Require Import Monad.
 From ConCert.Execution Require Import ResultMonad.
@@ -8,4 +9,61 @@ From ConCert.Execution Require Import Serializable.
 From ConCert.Utils Require Import RecordUpdate.
 
 Section Auction.
+  Context `{Base : ChainBase}.
+
+  Set Nonrecursive Elimination Schemes.
   
+  Inductive AuctionState :=
+  | not_sold_yet : AuctionState
+  | sold : AuctionState.
+
+  (** 
+      /// Type of the parameter to the `init` function
+      #[derive(Serialize, SchemaType)]
+      struct InitParameter {
+      /// The item to be sold
+      item:          String,
+      /// Time when auction ends using the RFC 3339 format (https://tools.ietf.org/html/rfc3339)
+      end:           Timestamp,
+      /// The minimum accepted raise to over bid the current bidder in Euro cent.
+      minimum_raise: u64,
+      }
+   *)
+  Record Setup :=
+    setup {
+        setup_seller : Address;
+        setup_item : string;
+        setup_duration : nat;
+        setup_minimum_raise : nat;
+      }.
+  
+  Record State :=
+    build_state {
+        auction_state : AuctionState;
+        seller : Address;
+        item : string;
+        duration : nat;
+        minimum_raise : nat;
+        highest_bidder : option Address;
+        last_action: nat;
+      }.
+
+  Definition Error : Type := nat.
+  Definition default_error: Error := 1%nat.
+
+  Inductive Msg := .
+
+  MetaCoq Run (make_setters State).
+
+  
+  Section Serialization.
+    Global Instance Setup_serializable : Serializable Setup :=
+      Derive Serializable Setup_rect<setup>.
+    
+    Global Instance AuctionState_serializable : Serializable AuctionState :=
+      Derive Serializable AuctionState_rect<not_sold_yet, sold>.
+    
+    Global Instance State_serializable : Serializable State :=
+      Derive Serializable State_rect<build_state>.
+  
+  End Serialization.
